{
"cells": [
{"cell_type":    "code", "execution_count":null, "metadata":{}, "source":["%%html\n<link href=\"http://mathbook.pugetsound.edu/beta/mathbook-content.css\" rel=\"stylesheet\" type=\"text/css\" />\n<link href=\"https://aimath.org/mathbook/mathbook-add-on.css\" rel=\"stylesheet\" type=\"text/css\" />\n<style>.subtitle {font-size:medium; display:block}</style>\n<link href=\"https://fonts.googleapis.com/css?family=Open+Sans:400,400italic,600,600italic\" rel=\"stylesheet\" type=\"text/css\" />\n<link href=\"https://fonts.googleapis.com/css?family=Inconsolata:400,700&subset=latin,latin-ext\" rel=\"stylesheet\" type=\"text/css\" /><!-- Hide this cell. -->\n<script>\nvar cell = $(\".container .cell\").eq(0), ia = cell.find(\".input_area\")\nif (cell.find(\".toggle-button\").length == 0) {\nia.after(\n    $('<button class=\"toggle-button\">Toggle hidden code</button>').click(\n        function (){ ia.toggle() }\n        )\n    )\nia.hide()\n}\n</script>\n"], "outputs":[]},
{"cell_type":"markdown", "metadata":{}, "source":["**Important:** to view this notebook properly you will need to execute the cell above, which assumes you have an Internet connection.  It should already be selected, or place your cursor anywhere above to select.  Then press the \"Run\" button in the menu bar above (the right-pointing arrowhead), or press Shift-Enter on your keyboard."]},
{"cell_type":"markdown", "metadata":{}, "source":["$\\newcommand{\\identity}{\\mathrm{id}}\n\\newcommand{\\notdivide}{\\nmid}\n\\newcommand{\\notsubset}{\\not\\subset}\n\\newcommand{\\lcm}{\\operatorname{lcm}}\n\\newcommand{\\gf}{\\operatorname{GF}}\n\\newcommand{\\inn}{\\operatorname{Inn}}\n\\newcommand{\\aut}{\\operatorname{Aut}}\n\\newcommand{\\Hom}{\\operatorname{Hom}}\n\\newcommand{\\cis}{\\operatorname{cis}}\n\\newcommand{\\chr}{\\operatorname{char}}\n\\newcommand{\\Null}{\\operatorname{Null}}\n\\newcommand{\\lt}{<}\n\\newcommand{\\gt}{>}\n\\newcommand{\\amp}{&}\n$"]},
{"cell_type":"markdown", "metadata":{}, "source":["<div class=\"mathbook-content\"><h2 class=\"heading hide-type\" alt=\"Exercises 17.5 Additional Exercises:  Solving the Cubic and Quartic Equations\"><span class=\"type\">Section</span><span class=\"codenumber\">17.5</span><span class=\"title\">Additional Exercises:  Solving the Cubic and Quartic Equations</span></h2><a href=\"poly-exercises-cubics-quartics.ipynb\" class=\"permalink\">¶</a></div>"]},
{"cell_type":"markdown", "metadata":{}, "source":["<div class=\"mathbook-content\"><article class=\"exercise-like\" id=\"exercise-608\"><h6 class=\"heading\"><span class=\"codenumber\">1</span></h6><p id=\"p-2695\">Solve the general quadratic equation</p><div class=\"displaymath\">\n\\begin{equation*}\nax^2 + bx + c = 0\n\\end{equation*}\n</div><p>to obtain</p><div class=\"displaymath\">\n\\begin{equation*}\nx = \\frac{-b \\pm \\sqrt{b^2 - 4ac}}{2a}.\n\\end{equation*}\n</div><p>The <dfn class=\"terminology\">discriminant</dfn> of the quadratic equation $\\Delta = b^2 - 4ac$ determines the nature of the solutions of the equation.  If $\\Delta \\gt 0\\text{,}$ the equation has two distinct real solutions.  If $\\Delta = 0\\text{,}$ the equation has a single repeated real root. If $\\Delta \\lt 0\\text{,}$ there are two distinct imaginary solutions.</p></article></div>"]},
{"cell_type":"markdown", "metadata":{}, "source":["<div class=\"mathbook-content\"><article class=\"exercise-like\" id=\"exercise-609\"><h6 class=\"heading\"><span class=\"codenumber\">2</span></h6><p id=\"p-2696\">Show that any cubic equation of the form</p><div class=\"displaymath\">\n\\begin{equation*}\nx^3 + bx^2 + cx + d = 0\n\\end{equation*}\n</div><p>can be reduced to the form $y^3 + py + q = 0$ by making the substitution $x = y - b/3\\text{.}$</p></article></div>"]},
{"cell_type":"markdown", "metadata":{}, "source":["<div class=\"mathbook-content\"><article class=\"exercise-like\" id=\"exercise-610\"><h6 class=\"heading\"><span class=\"codenumber\">3</span></h6><p id=\"p-2697\">Prove that the cube roots of 1 are given by</p><div class=\"displaymath\">\n\\begin{align*}\n\\omega & = \\frac{-1+ i \\sqrt{3}}{2}\\\\\n\\omega^2 & = \\frac{-1- i \\sqrt{3}}{2}\\\\\n\\omega^3 & = 1.\n\\end{align*}\n</div></article></div>"]},
{"cell_type":"markdown", "metadata":{}, "source":["<div class=\"mathbook-content\"><article class=\"exercise-like\" id=\"exercise-611\"><h6 class=\"heading\"><span class=\"codenumber\">4</span></h6><p id=\"p-2698\">Make the substitution</p><div class=\"displaymath\">\n\\begin{equation*}\ny = z - \\frac{p}{3 z}\n\\end{equation*}\n</div><p>for $y$ in the equation $y^3 + py + q = 0$ and obtain two solutions $A$ and $B$ for $z^3\\text{.}$</p></article></div>"]},
{"cell_type":"markdown", "metadata":{}, "source":["<div class=\"mathbook-content\"><article class=\"exercise-like\" id=\"exercise-612\"><h6 class=\"heading\"><span class=\"codenumber\">5</span></h6><p id=\"p-2699\">Show that the product of the solutions obtained in (4) is $-p^3/27\\text{,}$ deducing that $\\sqrt[3]{A B} = -p/3\\text{.}$</p></article></div>"]},
{"cell_type":"markdown", "metadata":{}, "source":["<div class=\"mathbook-content\"><article class=\"exercise-like\" id=\"exercise-613\"><h6 class=\"heading\"><span class=\"codenumber\">6</span></h6><p id=\"p-2700\">Prove that the possible solutions for $z$ in (4) are given by</p><div class=\"displaymath\">\n\\begin{equation*}\n\\sqrt[3]{A}, \\quad \\omega \\sqrt[3]{A}, \\quad \\omega^2 \\sqrt[3]{A}, \\quad \\sqrt[3]{B}, \\quad \\omega \\sqrt[3]{B}, \\quad \\omega^2 \\sqrt[3]{B}\n\\end{equation*}\n</div><p>and use this result to show that the three possible solutions for $y$ are</p><div class=\"displaymath\">\n\\begin{equation*}\n\\omega^i \\sqrt[3]{-\\frac{q}{2}+ \\sqrt{\\ \\frac{p^3}{27}  + \\frac{q^2}{4}}  } + \\omega^{2i} \\sqrt[3]{-\\frac{q}{2}- \\sqrt{\\ \\frac{p^3}{27}  + \\frac{q^2}{4}}  },\n\\end{equation*}\n</div><p>where $i = 0, 1, 2\\text{.}$</p></article></div>"]},
{"cell_type":"markdown", "metadata":{}, "source":["<div class=\"mathbook-content\"><article class=\"exercise-like\" id=\"exercise-614\"><h6 class=\"heading\"><span class=\"codenumber\">7</span></h6><p id=\"p-2701\">The <dfn class=\"terminology\">discriminant</dfn> of the cubic equation is</p><div class=\"displaymath\">\n\\begin{equation*}\n\\Delta = \\frac{p^3}{27}  + \\frac{q^2}{4}.\n\\end{equation*}\n</div><p>Show that $y^3 + py + q=0$ </p><ol class=\"lower-alpha\"><li id=\"li-606\"><p id=\"p-2702\">has three real roots, at least two of which are equal, if $\\Delta = 0\\text{.}$</p></li><li id=\"li-607\"><p id=\"p-2703\">has one real root and two conjugate imaginary roots if $\\Delta \\gt 0\\text{.}$</p></li><li id=\"li-608\"><p id=\"p-2704\">has three distinct real roots if $\\Delta \\lt 0\\text{.}$</p></li></ol></article></div>"]},
{"cell_type":"markdown", "metadata":{}, "source":["<div class=\"mathbook-content\"><article class=\"exercise-like\" id=\"exercise-615\"><h6 class=\"heading\"><span class=\"codenumber\">8</span></h6><p id=\"p-2705\">Solve the following cubic equations. </p><ol class=\"lower-alpha\"><li id=\"li-609\"><p id=\"p-2706\">$x^3 - 4x^2 + 11 x + 30 = 0$</p></li><li id=\"li-610\"><p id=\"p-2707\">$x^3 - 3x +5 = 0$</p></li><li id=\"li-611\"><p id=\"p-2708\">$x^3 - 3x +2 = 0$</p></li><li id=\"li-612\"><p id=\"p-2709\">$x^3 + x + 3 = 0$</p></li></ol></article></div>"]},
{"cell_type":"markdown", "metadata":{}, "source":["<div class=\"mathbook-content\"><article class=\"exercise-like\" id=\"exercise-616\"><h6 class=\"heading\"><span class=\"codenumber\">9</span></h6><p id=\"p-2710\">Show that the general quartic equation</p><div class=\"displaymath\">\n\\begin{equation*}\nx^4 + ax^3 + bx^2 + cx + d = 0\n\\end{equation*}\n</div><p>can be reduced to</p><div class=\"displaymath\">\n\\begin{equation*}\ny^4 + py^2 + qy + r = 0\n\\end{equation*}\n</div><p>by using the substitution $x = y - a/4\\text{.}$</p></article></div>"]},
{"cell_type":"markdown", "metadata":{}, "source":["<div class=\"mathbook-content\"><article class=\"exercise-like\" id=\"exercise-cubic-poly-10\"><h6 class=\"heading\"><span class=\"codenumber\">10</span></h6><p id=\"p-2711\">Show that</p><div class=\"displaymath\">\n\\begin{equation*}\n\\left( y^2 + \\frac{1}{2} z \\right)^2 = (z - p)y^2 - qy +  \\left( \\frac{1}{4} z^2 - r \\right).\n\\end{equation*}\n</div></article></div>"]},
{"cell_type":"markdown", "metadata":{}, "source":["<div class=\"mathbook-content\"><article class=\"exercise-like\" id=\"exercise-cubic-poly-11\"><h6 class=\"heading\"><span class=\"codenumber\">11</span></h6><p id=\"p-2712\">Show that the right-hand side of Exercise <a href=\"poly-exercises-cubics-quartics.ipynb#exercise-cubic-poly-10\" class=\"xref\" alt=\"Exercise 17.5.10 \" title=\"Exercise 17.5.10 \">17.5.10</a> can be put in the form $(my + k)^2$ if and only if</p><div class=\"displaymath\">\n\\begin{equation*}\nq^2 - 4(z - p)\\left( \\frac{1}{4} z^2 - r \\right) = 0.\n\\end{equation*}\n</div></article></div>"]},
{"cell_type":"markdown", "metadata":{}, "source":["<div class=\"mathbook-content\"><article class=\"exercise-like\" id=\"exercise-619\"><h6 class=\"heading\"><span class=\"codenumber\">12</span></h6><p id=\"p-2713\">From Exercise <a href=\"poly-exercises-cubics-quartics.ipynb#exercise-cubic-poly-11\" class=\"xref\" alt=\"Exercise 17.5.11 \" title=\"Exercise 17.5.11 \">17.5.11</a> obtain the <dfn class=\"terminology\">resolvent cubic equation</dfn></p><div class=\"displaymath\">\n\\begin{equation*}\nz^3 - pz^2 - 4rz + (4pr - q^2) = 0.\n\\end{equation*}\n</div><p>Solving the resolvent cubic equation, put the equation found in Exercise <a href=\"poly-exercises-cubics-quartics.ipynb#exercise-cubic-poly-10\" class=\"xref\" alt=\"Exercise 17.5.10 \" title=\"Exercise 17.5.10 \">17.5.10</a> in the form</p><div class=\"displaymath\">\n\\begin{equation*}\n\\left( y^2 + \\frac{1}{2} z \\right)^2 = (my + k)^2\n\\end{equation*}\n</div><p>to obtain the solution of the quartic equation.</p></article></div>"]},
{"cell_type":"markdown", "metadata":{}, "source":["<div class=\"mathbook-content\"><article class=\"exercise-like\" id=\"exercise-620\"><h6 class=\"heading\"><span class=\"codenumber\">13</span></h6><p id=\"p-2714\">Use this method to solve the following quartic equations. </p><ol class=\"lower-alpha\"><li id=\"li-613\"><p id=\"p-2715\">$x^4 - x^2 - 3x + 2 = 0$</p></li><li id=\"li-614\"><p id=\"p-2716\">$x^4 +  x^3 - 7 x^2 - x + 6 = 0$</p></li><li id=\"li-615\"><p id=\"p-2717\">$x^4 -2 x^2 + 4 x -3 = 0$</p></li><li id=\"li-616\"><p id=\"p-2718\">$x^4 - 4 x^3 + 3x^2 - 5x +2 = 0$</p></li></ol></article></div>"]}
],
"nbformat": 4, "nbformat_minor": 0, "metadata": {"kernelspec": {"display_name": "", "name": "sagemath"}, "language_info": {"codemirror_mode": {"name": "ipython", "version": 2}, "file_extension": ".py", "mimetype": "text/x-python", "name": "python", "nbconvert_exporter": "python", "pygments_lexer": "ipython2", "version": "2.7.8"}, "name": "poly-exercises-cubics-quartics.ipynb"}
}