{
"cells": [
{"cell_type":    "code", "execution_count":null, "metadata":{}, "source":["%%html\n<link href=\"http://mathbook.pugetsound.edu/beta/mathbook-content.css\" rel=\"stylesheet\" type=\"text/css\" />\n<link href=\"https://aimath.org/mathbook/mathbook-add-on.css\" rel=\"stylesheet\" type=\"text/css\" />\n<style>.subtitle {font-size:medium; display:block}</style>\n<link href=\"https://fonts.googleapis.com/css?family=Open+Sans:400,400italic,600,600italic\" rel=\"stylesheet\" type=\"text/css\" />\n<link href=\"https://fonts.googleapis.com/css?family=Inconsolata:400,700&subset=latin,latin-ext\" rel=\"stylesheet\" type=\"text/css\" /><!-- Hide this cell. -->\n<script>\nvar cell = $(\".container .cell\").eq(0), ia = cell.find(\".input_area\")\nif (cell.find(\".toggle-button\").length == 0) {\nia.after(\n    $('<button class=\"toggle-button\">Toggle hidden code</button>').click(\n        function (){ ia.toggle() }\n        )\n    )\nia.hide()\n}\n</script>\n"], "outputs":[]},
{"cell_type":"markdown", "metadata":{}, "source":["**Important:** to view this notebook properly you will need to execute the cell above, which assumes you have an Internet connection.  It should already be selected, or place your cursor anywhere above to select.  Then press the \"Run\" button in the menu bar above (the right-pointing arrowhead), or press Shift-Enter on your keyboard."]},
{"cell_type":"markdown", "metadata":{}, "source":["$\\newcommand{\\identity}{\\mathrm{id}}\n\\newcommand{\\notdivide}{\\nmid}\n\\newcommand{\\notsubset}{\\not\\subset}\n\\newcommand{\\lcm}{\\operatorname{lcm}}\n\\newcommand{\\gf}{\\operatorname{GF}}\n\\newcommand{\\inn}{\\operatorname{Inn}}\n\\newcommand{\\aut}{\\operatorname{Aut}}\n\\newcommand{\\Hom}{\\operatorname{Hom}}\n\\newcommand{\\cis}{\\operatorname{cis}}\n\\newcommand{\\chr}{\\operatorname{char}}\n\\newcommand{\\Null}{\\operatorname{Null}}\n\\newcommand{\\lt}{<}\n\\newcommand{\\gt}{>}\n\\newcommand{\\amp}{&}\n$"]},
{"cell_type":"markdown", "metadata":{}, "source":["<div class=\"mathbook-content\"><h2 class=\"heading hide-type\" alt=\"Section 17.1 Polynomial Rings\"><span class=\"type\">Section</span><span class=\"codenumber\">17.1</span><span class=\"title\">Polynomial Rings</span></h2><a href=\"section-poly-rings.ipynb\" class=\"permalink\">¶</a></div>"]},
{"cell_type":"markdown", "metadata":{}, "source":["<div class=\"mathbook-content\"><p id=\"p-2564\">Throughout this chapter we shall assume that $R$ is a commutative ring with identity.  Any expression of the form</p><div class=\"displaymath\">\n\\begin{equation*}\nf(x) = \\sum^{n}_{i=0} a_i x^i = a_0 + a_1 x +a_2 x^2 + \\cdots + a_n x^n,\n\\end{equation*}\n</div><p>where $a_i \\in R$ and $a_n \\neq 0\\text{,}$ is called a <dfn class=\"terminology\">polynomial over $R$</dfn> with <dfn class=\"terminology\">indeterminate</dfn> $x\\text{.}$  The elements $a_0, a_1, \\ldots, a_n$ are called the <dfn class=\"terminology\">coefficients</dfn> of $f\\text{.}$  The coefficient $a_n$ is called the <dfn class=\"terminology\">leading coefficient</dfn>.  A polynomial is called <dfn class=\"terminology\">monic</dfn> if the leading coefficient is 1.  If $n$ is the largest nonnegative number for which $a_n \\neq 0\\text{,}$ we say that the <dfn class=\"terminology\">degree</dfn> of $f$ is $n$ and write $\\deg f(x) = n\\text{.}$    If no such $n$ exists—that is, if $f=0$ is the zero polynomial—then the degree of $f$ is defined to be $-\\infty\\text{.}$  We will denote the set of all polynomials with coefficients in a ring $R$ by $R[x]\\text{.}$    Two polynomials are equal exactly when their corresponding coefficients are equal; that is, if we let</p><div class=\"displaymath\">\n\\begin{align*}\np(x) & = a_0 + a_1 x + \\cdots + a_n x^n\\\\\nq(x) & = b_0 + b_1 x + \\cdots + b_m x^m,\n\\end{align*}\n</div><p>then $p(x) = q(x)$ if and only if $a_i = b_i$ for all $i \\geq 0\\text{.}$</p></div>"]},
{"cell_type":"markdown", "metadata":{}, "source":["<div class=\"mathbook-content\"><p id=\"p-2565\">To show that the set of all polynomials forms a ring, we must first define addition and multiplication.  We define the sum of two polynomials as follows.  Let</p><div class=\"displaymath\">\n\\begin{align*}\np(x) & = a_0 + a_1 x + \\cdots + a_n x^n\\\\\nq(x) & = b_0 + b_1 x + \\cdots + b_m x^m.\n\\end{align*}\n</div><p>Then the sum of $p(x)$ and $q(x)$ is</p><div class=\"displaymath\">\n\\begin{equation*}\np(x) + q(x) = c_0 + c_1 x + \\cdots + c_k x^k,\n\\end{equation*}\n</div><p>where $c_i = a_i + b_i$ for each $i\\text{.}$  We define the product of $p(x)$ and $q(x)$ to be</p><div class=\"displaymath\">\n\\begin{equation*}\np(x) q(x) = c_0 + c_1 x + \\cdots + c_{m + n} x^{m + n},\n\\end{equation*}\n</div><p>where</p><div class=\"displaymath\">\n\\begin{equation*}\nc_i = \\sum_{k = 0}^i a_k b_{i - k} = a_0  b_i + a_1 b_{i -1} + \\cdots + a_{i -1} b _1 + a_i b_0\n\\end{equation*}\n</div><p>for each $i\\text{.}$  Notice that in each case some of the coefficients may be zero.</p></div>"]},
{"cell_type":"markdown", "metadata":{}, "source":["<div class=\"mathbook-content\"><article class=\"example-like\" id=\"example-poly-operations\"><h6 class=\"heading\"><span class=\"type\">Example</span><span class=\"codenumber\">17.1</span></h6><p id=\"p-2566\">Suppose that</p><div class=\"displaymath\">\n\\begin{equation*}\np(x) = 3 + 0 x + 0 x^2 + 2 x^3 + 0 x^4\n\\end{equation*}\n</div><p>and</p><div class=\"displaymath\">\n\\begin{equation*}\nq(x) = 2 + 0 x - x^2 + 0 x^3 + 4 x^4\n\\end{equation*}\n</div><p>are polynomials in ${\\mathbb Z}[x]\\text{.}$  If the coefficient of some term in a polynomial is zero, then we usually just omit that term.  In this case we  would write $p(x) =  3 + 2 x^3$ and $q(x) = 2 - x^2 + 4 x^4\\text{.}$  The sum of these two polynomials is</p><div class=\"displaymath\">\n\\begin{equation*}\np(x) + q(x)= 5 - x^2 + 2 x^3 + 4 x^4.\n\\end{equation*}\n</div><p>The product,</p><div class=\"displaymath\">\n\\begin{equation*}\np(x) q(x) = (3 + 2 x^3)( 2 - x^2 + 4 x^4 ) =  6 - 3x^2 + 4 x^3 + 12 x^4  - 2 x^5 + 8 x^7,\n\\end{equation*}\n</div><p>can be calculated either by determining the $c_i$'s in the definition or by simply multiplying polynomials in the same way as we have always done.</p></article></div>"]},
{"cell_type":"markdown", "metadata":{}, "source":["<div class=\"mathbook-content\"><article class=\"example-like\" id=\"example-poly-integral-domains\"><h6 class=\"heading\"><span class=\"type\">Example</span><span class=\"codenumber\">17.2</span></h6><p id=\"p-2567\">Let</p><div class=\"displaymath\">\n\\begin{equation*}\np(x) = 3 + 3 x^3 \\qquad \\text{and} \\qquad q(x) = 4 + 4 x^2 + 4 x^4\n\\end{equation*}\n</div><p>be polynomials in ${\\mathbb Z}_{12}[x]\\text{.}$ The sum of $p(x)$ and $q(x)$ is $7 + 4 x^2 + 3 x^3 + 4 x^4\\text{.}$  The product of the two polynomials is  the zero polynomial.  This example tells us that we can not expect $R[x]$ to be an integral domain if $R$ is not an integral domain.</p></article></div>"]},
{"cell_type":"markdown", "metadata":{}, "source":["<div class=\"mathbook-content\"><article class=\"theorem-like\" id=\"theorem-poly-1\"><h6 class=\"heading\"><span class=\"type\">Theorem</span><span class=\"codenumber\">17.3</span></h6><p id=\"p-2568\">Let $R$ be a commutative ring with identity.  Then $R[x]$ is a commutative ring with identity.</p></article><article class=\"proof\" id=\"proof-116\"><h6 class=\"heading\"><span class=\"type\">Proof</span></h6><p id=\"p-2569\">Our first task is to show that $R[x]$ is an abelian group under polynomial addition.  The zero polynomial, $f(x) = 0\\text{,}$ is the additive identity.  Given a polynomial $p(x) = \\sum_{i = 0}^{n} a_i x^i\\text{,}$ the inverse of $p(x)$ is easily verified to be $-p(x) = \\sum_{i = 0}^{n} (-a_i) x^i = -\\sum_{i = 0}^{n} a_i x^i\\text{.}$  Commutativity and associativity follow immediately from the definition of polynomial addition and from the fact that addition in $R$ is both commutative and associative.</p><p id=\"p-2570\">To show that polynomial multiplication is associative, let</p><div class=\"displaymath\">\n\\begin{align*}\np(x) & = \\sum_{i = 0}^{m} a_i x^i,\\\\\nq(x) & = \\sum_{i = 0}^{n} b_i x^i,\\\\\nr(x) & = \\sum_{i = 0}^{p} c_i x^i.\n\\end{align*}\n</div><p>Then</p><div class=\"displaymath\">\n\\begin{align*}\n[p(x) q(x)] r(x) & = \\left[ \\left( \\sum_{i=0}^{m} a_i x^i  \\right) \\left(  \\sum_{i=0}^{n} b_i x^i \\right) \\right] \\left( \\sum_{i = 0}^{p} c_i x^i \\right)\\\\\n& = \\left[ \\sum_{i = 0}^{m+n} \\left(  \\sum_{j = 0}^{i} a_j b_{i - j} \\right) x^i \\right] \\left( \\sum_{i = 0}^{p} c_i x^i \\right)\\\\\n& = \\sum_{i = 0}^{m + n + p} \\left[ \\sum_{j = 0}^{i} \\left( \\sum_{k=0}^j a_k b_{j-k} \\right) c_{i-j} \\right] x^i\\\\\n& = \\sum_{i = 0}^{m + n + p} \\left(\\sum_{j + k + l = i} a_j b_k c_l \\right) x^i\\\\\n& = \\sum_{i = 0}^{m+n+p} \\left[ \\sum_{j = 0}^{i} a_j  \\left( \\sum_{k = 0}^{i - j} b_k c_{i - j - k} \\right) \\right]  x^i\\\\\n& = \\left( \\sum_{i = 0}^{m} a_i x^i  \\right) \\left[ \\sum_{i = 0}^{n + p}  \\left( \\sum_{j = 0}^{i} b_j c_{i - j} \\right) x^i \\right]\\\\\n& = \\left( \\sum_{i = 0}^{m} a_i x^i \\right) \\left[ \\left(  \\sum_{i = 0}^{n} b_i x^i \\right) \\left( \\sum_{i = 0}^{p} c_i x^i \\right) \\right]\\\\\n& = p(x) [ q(x) r(x) ]\n\\end{align*}\n</div><p>The commutativity and distribution properties of polynomial multiplication are proved in a similar manner.  We shall leave the proofs of these properties as an exercise.</p></article></div>"]},
{"cell_type":"markdown", "metadata":{}, "source":["<div class=\"mathbook-content\"><article class=\"theorem-like\" id=\"proposition-poly-integral-domain\"><h6 class=\"heading\"><span class=\"type\">Proposition</span><span class=\"codenumber\">17.4</span></h6><p id=\"p-2571\">Let $p(x)$ and $q(x)$ be polynomials in $R[x]\\text{,}$ where $R$ is an integral domain.  Then $\\deg p(x) + \\deg q(x) = \\deg( p(x) q(x) )\\text{.}$  Furthermore, $R[x]$ is an integral domain.</p></article><article class=\"proof\" id=\"proof-117\"><h6 class=\"heading\"><span class=\"type\">Proof</span></h6><p id=\"p-2572\">Suppose that we have two nonzero polynomials</p><div class=\"displaymath\">\n\\begin{equation*}\np(x) = a_m x^m + \\cdots + a_1 x + a_0\n\\end{equation*}\n</div><p>and</p><div class=\"displaymath\">\n\\begin{equation*}\nq(x) = b_n x^n + \\cdots + b_1 x + b_0\n\\end{equation*}\n</div><p>with $a_m \\neq 0$ and $b_n \\neq 0\\text{.}$ The degrees of $p(x)$ and $q(x)$ are $m$ and $n\\text{,}$ respectively.  The leading term of $p(x) q(x)$ is $a_m b_n x^{m + n}\\text{,}$ which cannot be zero since $R$ is an integral domain; hence, the degree of $p(x) q(x)$ is $m + n\\text{,}$ and $p(x)q(x) \\neq 0\\text{.}$  Since $p(x) \\neq 0$ and $q(x) \\neq 0$ imply that $p(x)q(x) \\neq 0\\text{,}$ we know that $R[x]$ must also be an integral domain.</p></article></div>"]},
{"cell_type":"markdown", "metadata":{}, "source":["<div class=\"mathbook-content\"><p id=\"p-2573\">We also want to consider polynomials in two or more variables, such as $x^2 - 3 x y + 2 y^3\\text{.}$  Let $R$ be a ring and suppose that we are given two indeterminates $x$ and $y\\text{.}$  Certainly we can form the ring $(R[x])[y]\\text{.}$  It is straightforward but perhaps tedious to show that $(R[x])[y] \\cong R([y])[x]\\text{.}$  We shall identify these two rings by this isomorphism and simply write $R[x,y]\\text{.}$  The ring $R[x, y]$ is called the <dfn class=\"terminology\">ring of polynomials in two indeterminates $x$ and $y$ with coefficients in</dfn> $R\\text{.}$  We can define the <dfn class=\"terminology\">ring of polynomials in</dfn> $n$ <dfn class=\"terminology\">indeterminates with coefficients in</dfn> $R$ similarly.  We shall denote this ring by $R[x_1, x_2, \\ldots, x_n]\\text{.}$ </p></div>"]},
{"cell_type":"markdown", "metadata":{}, "source":["<div class=\"mathbook-content\"><article class=\"theorem-like\" id=\"theorem-poly-3\"><h6 class=\"heading\"><span class=\"type\">Theorem</span><span class=\"codenumber\">17.5</span></h6><p id=\"p-2574\">Let $R$ be a commutative ring with identity and $\\alpha \\in R\\text{.}$  Then we have a ring homomorphism  $\\phi_{\\alpha} : R[x] \\rightarrow R$ defined by </p><div class=\"displaymath\">\n\\begin{equation*}\n\\phi_{\\alpha} (p(x) ) = p( \\alpha ) = a_n \\alpha^n + \\cdots + a_1 \\alpha + a_0,\n\\end{equation*}\n</div><p>where $p( x ) = a_n x^n + \\cdots + a_1 x + a_0\\text{.}$</p></article><article class=\"proof\" id=\"proof-118\"><h6 class=\"heading\"><span class=\"type\">Proof</span></h6><p id=\"p-2575\">Let $p(x) = \\sum_{i = 0}^n a_i x^i$ and $q(x) = \\sum_{i = 0}^m b_i x^i\\text{.}$  It is easy to show that $\\phi_{\\alpha}(p(x) + q(x)) = \\phi_{\\alpha}(p(x))  + \\phi_{\\alpha}(q(x))\\text{.}$  To show that multiplication is preserved under the map $\\phi_{\\alpha}\\text{,}$ observe that</p><div class=\"displaymath\">\n\\begin{align*}\n\\phi_{\\alpha} (p(x) ) \\phi_{\\alpha} (q(x)) & = p( \\alpha ) q(\\alpha)\\\\\n& = \\left( \\sum_{i = 0}^n a_i \\alpha^i \\right) \\left( \\sum_{i = 0}^m b_i \\alpha^i \\right)\\\\\n& = \\sum_{i = 0}^{m + n} \\left( \\sum_{k = 0}^i a_k b_{i - k} \\right) \\alpha^i\\\\\n& = \\phi_{\\alpha} (p(x) q(x)).\n\\end{align*}\n</div></article></div>"]},
{"cell_type":"markdown", "metadata":{}, "source":["<div class=\"mathbook-content\"><p id=\"p-2576\">The map  $\\phi_{\\alpha} : R[x] \\rightarrow R$ is called the <dfn class=\"terminology\">evaluation homomorphism</dfn> at $\\alpha\\text{.}$</p></div>"]}
],
"nbformat": 4, "nbformat_minor": 0, "metadata": {"kernelspec": {"display_name": "", "name": "sagemath"}, "language_info": {"codemirror_mode": {"name": "ipython", "version": 2}, "file_extension": ".py", "mimetype": "text/x-python", "name": "python", "nbconvert_exporter": "python", "pygments_lexer": "ipython2", "version": "2.7.8"}, "name": "section-poly-rings.ipynb"}
}