{
"cells": [
{"cell_type":    "code", "execution_count":null, "metadata":{}, "source":["%%html\n<link href=\"http://mathbook.pugetsound.edu/beta/mathbook-content.css\" rel=\"stylesheet\" type=\"text/css\" />\n<link href=\"https://aimath.org/mathbook/mathbook-add-on.css\" rel=\"stylesheet\" type=\"text/css\" />\n<style>.subtitle {font-size:medium; display:block}</style>\n<link href=\"https://fonts.googleapis.com/css?family=Open+Sans:400,400italic,600,600italic\" rel=\"stylesheet\" type=\"text/css\" />\n<link href=\"https://fonts.googleapis.com/css?family=Inconsolata:400,700&subset=latin,latin-ext\" rel=\"stylesheet\" type=\"text/css\" /><!-- Hide this cell. -->\n<script>\nvar cell = $(\".container .cell\").eq(0), ia = cell.find(\".input_area\")\nif (cell.find(\".toggle-button\").length == 0) {\nia.after(\n    $('<button class=\"toggle-button\">Toggle hidden code</button>').click(\n        function (){ ia.toggle() }\n        )\n    )\nia.hide()\n}\n</script>\n"], "outputs":[]},
{"cell_type":"markdown", "metadata":{}, "source":["**Important:** to view this notebook properly you will need to execute the cell above, which assumes you have an Internet connection.  It should already be selected, or place your cursor anywhere above to select.  Then press the \"Run\" button in the menu bar above (the right-pointing arrowhead), or press Shift-Enter on your keyboard."]},
{"cell_type":"markdown", "metadata":{}, "source":["$\\newcommand{\\identity}{\\mathrm{id}}\n\\newcommand{\\notdivide}{\\nmid}\n\\newcommand{\\notsubset}{\\not\\subset}\n\\newcommand{\\lcm}{\\operatorname{lcm}}\n\\newcommand{\\gf}{\\operatorname{GF}}\n\\newcommand{\\inn}{\\operatorname{Inn}}\n\\newcommand{\\aut}{\\operatorname{Aut}}\n\\newcommand{\\Hom}{\\operatorname{Hom}}\n\\newcommand{\\cis}{\\operatorname{cis}}\n\\newcommand{\\chr}{\\operatorname{char}}\n\\newcommand{\\Null}{\\operatorname{Null}}\n\\newcommand{\\lt}{<}\n\\newcommand{\\gt}{>}\n\\newcommand{\\amp}{&}\n$"]},
{"cell_type":"markdown", "metadata":{}, "source":["<div class=\"mathbook-content\"><h2 class=\"heading hide-type\" alt=\"Section 6.1 Cosets\"><span class=\"type\">Section</span><span class=\"codenumber\">6.1</span><span class=\"title\">Cosets</span></h2><a href=\"section-cosets.ipynb\" class=\"permalink\">¶</a></div>"]},
{"cell_type":"markdown", "metadata":{}, "source":["<div class=\"mathbook-content\"><p id=\"p-968\">Let $G$ be a group and $H$ a subgroup of $G\\text{.}$  Define a <dfn class=\"terminology\">left coset</dfn> of $H$ with <dfn class=\"terminology\">representative</dfn> $g \\in G$ to be the set</p><div class=\"displaymath\">\n\\begin{equation*}\ngH = \\{ gh : h \\in H \\}.\n\\end{equation*}\n</div><p><dfn class=\"terminology\">Right cosets</dfn> can be defined similarly by</p><div class=\"displaymath\">\n\\begin{equation*}\nHg = \\{ hg : h \\in H \\}.\n\\end{equation*}\n</div><p>If left and right cosets coincide or if it is clear from the context to which type of coset that we are referring, we will use the word <em class=\"emphasis\">coset</em> without specifying left or right.</p></div>"]},
{"cell_type":"markdown", "metadata":{}, "source":["<div class=\"mathbook-content\"><article class=\"example-like\" id=\"example-cosets-z6-cosets\"><h6 class=\"heading\"><span class=\"type\">Example</span><span class=\"codenumber\">6.1</span></h6><p id=\"p-969\">Let $H$ be the subgroup of ${\\mathbb Z}_6$ consisting of the elements 0 and 3.  The cosets are</p><div class=\"displaymath\">\n\\begin{gather*}\n0 + H = 3 + H = \\{ 0, 3 \\}\\\\\n1 + H = 4 + H = \\{ 1, 4 \\}\\\\\n2 + H = 5 + H = \\{ 2, 5 \\}.\n\\end{gather*}\n</div><p>We will always write the cosets of subgroups of ${\\mathbb Z}$ and ${\\mathbb Z}_n$ with the additive notation we have used for cosets here.  In a commutative group, left and right cosets are always identical.</p></article></div>"]},
{"cell_type":"markdown", "metadata":{}, "source":["<div class=\"mathbook-content\"><article class=\"example-like\" id=\"example-cosets-s3-cosets\"><h6 class=\"heading\"><span class=\"type\">Example</span><span class=\"codenumber\">6.2</span></h6><p id=\"p-970\">Let $H$ be the subgroup of $S_3$ defined by the permutations $\\{(1), (123), (132) \\}\\text{.}$  The left cosets of $H$ are</p><div class=\"displaymath\">\n\\begin{gather*}\n(1)H = (1 2 3)H =  (132)H = \\{(1), (1 23), (132) \\}\\\\\n(1 2)H = (1 3)H = (2 3)H =  \\{ (1 2), (1 3), (2 3)  \\}.\n\\end{gather*}\n</div><p>The right cosets of $H$ are exactly the same as the left cosets:</p><div class=\"displaymath\">\n\\begin{gather*}\nH(1) = H(1 2 3) =  H(132) = \\{(1), (1 23), (132) \\}\\\\\nH(1 2) = H(1 3) = H(2 3) =  \\{ (1 2), (1 3), (2 3)  \\}.\n\\end{gather*}\n</div><p id=\"p-971\">It is not always the case that a left coset is the same as a right coset.  Let $K$ be the subgroup of $S_3$ defined by the permutations $\\{(1), (1 2)\\}\\text{.}$  Then the left cosets of $K$ are</p><div class=\"displaymath\">\n\\begin{gather*}\n(1)K = (1 2)K = \\{(1), (1 2)\\}\\\\\n(1 3)K = (1 2 3)K = \\{(1 3), (1 2 3)\\}\\\\\n(2 3)K = (1 3 2)K = \\{(2 3), (1 3 2)\\};\n\\end{gather*}\n</div><p>however, the right cosets of $K$ are</p><div class=\"displaymath\">\n\\begin{gather*}\nK(1) = K(1 2) = \\{(1), (1 2)\\}\\\\\nK(1 3) = K(1 3 2) = \\{(1 3), (1 3 2)\\}\\\\\nK(2 3) = K(1 2 3) = \\{(2 3), (1 2 3)\\}.\n\\end{gather*}\n</div></article></div>"]},
{"cell_type":"markdown", "metadata":{}, "source":["<div class=\"mathbook-content\"><p id=\"p-972\">The following lemma is quite useful when dealing with cosets.  (We leave its proof as an exercise.)</p></div>"]},
{"cell_type":"markdown", "metadata":{}, "source":["<div class=\"mathbook-content\"><article class=\"theorem-like\" id=\"lemma-cosets-theorem-1\"><h6 class=\"heading\"><span class=\"type\">Lemma</span><span class=\"codenumber\">6.3</span></h6><p id=\"p-973\">Let $H$ be a subgroup of a group $G$ and suppose that $g_1, g_2 \\in G\\text{.}$  The following conditions are equivalent. </p><ol class=\"decimal\"><li id=\"li-253\"><p id=\"p-974\">$g_1 H = g_2 H\\text{;}$</p></li><li id=\"li-254\"><p id=\"p-975\">$H g_1^{-1}  = H g_2^{-1}\\text{;}$</p></li><li id=\"li-255\"><p id=\"p-976\">$g_1 H \\subset g_2 H\\text{;}$</p></li><li id=\"li-256\"><p id=\"p-977\">$g_2 \\in g_1 H\\text{;}$</p></li><li id=\"li-257\"><p id=\"p-978\">$g_1^{-1} g_2 \\in H\\text{.}$</p></li></ol></article></div>"]},
{"cell_type":"markdown", "metadata":{}, "source":["<div class=\"mathbook-content\"><p id=\"p-979\">In all of our  examples the cosets of a subgroup $H$ partition the larger group $G\\text{.}$  The following theorem proclaims that this will always be the case.</p></div>"]},
{"cell_type":"markdown", "metadata":{}, "source":["<div class=\"mathbook-content\"><article class=\"theorem-like\" id=\"theorem-cosets-theorem-2\"><h6 class=\"heading\"><span class=\"type\">Theorem</span><span class=\"codenumber\">6.4</span></h6><p id=\"p-980\">Let $H$ be a subgroup of a group $G\\text{.}$  Then the left cosets of $H$ in $G$ partition $G\\text{.}$  That is, the group $G$ is the disjoint union of the left cosets of $H$ in $G\\text{.}$</p></article><article class=\"proof\" id=\"proof-36\"><h6 class=\"heading\"><span class=\"type\">Proof</span></h6><p id=\"p-981\">Let $g_1 H$ and $g_2 H$ be two cosets of $H$ in $G\\text{.}$  We must show that either $g_1 H \\cap g_2 H = \\emptyset$ or $g_1 H = g_2 H\\text{.}$  Suppose that $g_1 H \\cap g_2 H \\neq \\emptyset$ and $a \\in g_1 H \\cap g_2 H\\text{.}$  Then by the definition of a left coset, $a = g_1 h_1 = g_2 h_2$ for some elements $h_1$ and $h_2$ in $H\\text{.}$  Hence, $g_1 = g_2 h_2 h_1^{-1}$ or $g_1 \\in g_2 H\\text{.}$  By Lemma <a href=\"section-cosets.ipynb#lemma-cosets-theorem-1\" class=\"xref\" alt=\"Lemma 6.3 \" title=\"Lemma 6.3 \">6.3</a>, $g_1 H = g_2 H\\text{.}$</p></article></div>"]},
{"cell_type":"markdown", "metadata":{}, "source":["<div class=\"mathbook-content\"><article class=\"remark-like\" id=\"remark-4\"><h6 class=\"heading\"><span class=\"type\">Remark</span><span class=\"codenumber\">6.5</span></h6><p id=\"p-982\">There is nothing special in this theorem about left cosets.  Right cosets also partition $G\\text{;}$ the proof of this fact is exactly the same as the proof for left cosets except that all group multiplications are done on the opposite side of $H\\text{.}$</p></article></div>"]},
{"cell_type":"markdown", "metadata":{}, "source":["<div class=\"mathbook-content\"><p id=\"p-983\">Let $G$ be a group and $H$ be a subgroup of $G\\text{.}$  Define the <dfn class=\"terminology\">index</dfn> of $H$ in $G$ to be the number of left cosets of $H$ in $G\\text{.}$  We will denote the index by $[G:H]\\text{.}$ </p></div>"]},
{"cell_type":"markdown", "metadata":{}, "source":["<div class=\"mathbook-content\"><article class=\"example-like\" id=\"example-cosets-z6-index\"><h6 class=\"heading\"><span class=\"type\">Example</span><span class=\"codenumber\">6.6</span></h6><p id=\"p-984\">Let $G= {\\mathbb Z}_6$ and $H = \\{ 0, 3 \\}\\text{.}$ Then $[G:H] = 3\\text{.}$</p></article></div>"]},
{"cell_type":"markdown", "metadata":{}, "source":["<div class=\"mathbook-content\"><article class=\"example-like\" id=\"example-cosets-s3-index\"><h6 class=\"heading\"><span class=\"type\">Example</span><span class=\"codenumber\">6.7</span></h6><p id=\"p-985\">Suppose that $G= S_3\\text{,}$ $H = \\{ (1),(123), (132) \\}\\text{,}$ and $K= \\{ (1), (12) \\}\\text{.}$  Then $[G:H] = 2$ and $[G:K] = 3\\text{.}$</p></article></div>"]},
{"cell_type":"markdown", "metadata":{}, "source":["<div class=\"mathbook-content\"><article class=\"theorem-like\" id=\"theorem-cosets-theorem-3\"><h6 class=\"heading\"><span class=\"type\">Theorem</span><span class=\"codenumber\">6.8</span></h6><p id=\"p-986\">Let $H$ be a subgroup of a group $G\\text{.}$  The number of left cosets of $H$ in $G$ is the same as the number of right cosets of $H$ in $G\\text{.}$</p></article><article class=\"proof\" id=\"proof-37\"><h6 class=\"heading\"><span class=\"type\">Proof</span></h6><p id=\"p-987\">Let ${\\mathcal L}_H$ and  ${\\mathcal R}_H$ denote the set of left and right cosets of $H$ in $G\\text{,}$ respectively.   If we can define a bijective map $\\phi :  {\\mathcal L}_H \\rightarrow {\\mathcal R}_H\\text{,}$ then the theorem will be proved.  If $gH \\in {\\mathcal L}_H\\text{,}$ let $\\phi( gH ) = Hg^{-1}\\text{.}$  By Lemma <a href=\"section-cosets.ipynb#lemma-cosets-theorem-1\" class=\"xref\" alt=\"Lemma 6.3 \" title=\"Lemma 6.3 \">6.3</a>, the map $\\phi$ is well-defined; that is, if $g_1 H = g_2 H\\text{,}$ then $H g_1^{-1} = H g_2^{-1}\\text{.}$  To show that $\\phi$ is one-to-one, suppose that</p><div class=\"displaymath\">\n\\begin{equation*}\nH g_1^{-1} = \\phi( g_1 H ) = \\phi( g_2 H ) = H g_2^{-1}.\n\\end{equation*}\n</div><p>Again by Lemma <a href=\"section-cosets.ipynb#lemma-cosets-theorem-1\" class=\"xref\" alt=\"Lemma 6.3 \" title=\"Lemma 6.3 \">6.3</a>, $g_1 H = g_2 H\\text{.}$  The map $\\phi$ is onto since $\\phi(g^{-1} H ) = H g\\text{.}$</p></article></div>"]}
],
"nbformat": 4, "nbformat_minor": 0, "metadata": {"kernelspec": {"display_name": "", "name": "sagemath"}, "language_info": {"codemirror_mode": {"name": "ipython", "version": 2}, "file_extension": ".py", "mimetype": "text/x-python", "name": "python", "nbconvert_exporter": "python", "pygments_lexer": "ipython2", "version": "2.7.8"}, "name": "section-cosets.ipynb"}
}