{
"cells": [
{"cell_type":    "code", "execution_count":null, "metadata":{}, "source":["%%html\n<link href=\"http://mathbook.pugetsound.edu/beta/mathbook-content.css\" rel=\"stylesheet\" type=\"text/css\" />\n<link href=\"https://aimath.org/mathbook/mathbook-add-on.css\" rel=\"stylesheet\" type=\"text/css\" />\n<style>.subtitle {font-size:medium; display:block}</style>\n<link href=\"https://fonts.googleapis.com/css?family=Open+Sans:400,400italic,600,600italic\" rel=\"stylesheet\" type=\"text/css\" />\n<link href=\"https://fonts.googleapis.com/css?family=Inconsolata:400,700&subset=latin,latin-ext\" rel=\"stylesheet\" type=\"text/css\" /><!-- Hide this cell. -->\n<script>\nvar cell = $(\".container .cell\").eq(0), ia = cell.find(\".input_area\")\nif (cell.find(\".toggle-button\").length == 0) {\nia.after(\n    $('<button class=\"toggle-button\">Toggle hidden code</button>').click(\n        function (){ ia.toggle() }\n        )\n    )\nia.hide()\n}\n</script>\n"], "outputs":[]},
{"cell_type":"markdown", "metadata":{}, "source":["**Important:** to view this notebook properly you will need to execute the cell above, which assumes you have an Internet connection.  It should already be selected, or place your cursor anywhere above to select.  Then press the \"Run\" button in the menu bar above (the right-pointing arrowhead), or press Shift-Enter on your keyboard."]},
{"cell_type":"markdown", "metadata":{}, "source":["$\\newcommand{\\identity}{\\mathrm{id}}\n\\newcommand{\\notdivide}{\\nmid}\n\\newcommand{\\notsubset}{\\not\\subset}\n\\newcommand{\\lcm}{\\operatorname{lcm}}\n\\newcommand{\\gf}{\\operatorname{GF}}\n\\newcommand{\\inn}{\\operatorname{Inn}}\n\\newcommand{\\aut}{\\operatorname{Aut}}\n\\newcommand{\\Hom}{\\operatorname{Hom}}\n\\newcommand{\\cis}{\\operatorname{cis}}\n\\newcommand{\\chr}{\\operatorname{char}}\n\\newcommand{\\Null}{\\operatorname{Null}}\n\\newcommand{\\lt}{<}\n\\newcommand{\\gt}{>}\n\\newcommand{\\amp}{&}\n$"]},
{"cell_type":"markdown", "metadata":{}, "source":["<div class=\"mathbook-content\"><h2 class=\"heading hide-type\" alt=\"Section 17.2 The Division Algorithm\"><span class=\"type\">Section</span><span class=\"codenumber\">17.2</span><span class=\"title\">The Division Algorithm</span></h2><a href=\"section-poly-division-algorithm.ipynb\" class=\"permalink\">¶</a></div>"]},
{"cell_type":"markdown", "metadata":{}, "source":["<div class=\"mathbook-content\"><p id=\"p-2577\">Recall that the division algorithm for integers (Theorem <a href=\"section-division-algorithm.ipynb#theorem-integers-division_algorithm\" class=\"xref\" alt=\"Theorem 2.9 Division Algorithm\" title=\"Theorem 2.9 Division Algorithm\">2.9</a>) says that if $a$ and $b$ are integers with $b \\gt 0\\text{,}$ then there exist unique integers $q$ and $r$ such that $a = bq+r\\text{,}$ where $0 \\leq r \\lt b\\text{.}$ The algorithm by which $q$ and $r$ are found is just long division.  A similar theorem exists for polynomials. The division algorithm for polynomials has several important consequences. Since its proof is very similar to the corresponding proof for integers, it is worthwhile to review Theorem <a href=\"section-division-algorithm.ipynb#theorem-integers-division_algorithm\" class=\"xref\" alt=\"Theorem 2.9 Division Algorithm\" title=\"Theorem 2.9 Division Algorithm\">2.9</a> at this point.</p></div>"]},
{"cell_type":"markdown", "metadata":{}, "source":["<div class=\"mathbook-content\"><article class=\"theorem-like\" id=\"theorem-90\"><h6 class=\"heading\"><span class=\"type\">Theorem</span><span class=\"codenumber\">17.6</span><span class=\"title\">Division Algorithm</span></h6><p id=\"p-2578\">Let $f(x)$ and $g(x)$ be polynomials in $F[x]\\text{,}$ where $F$ is a field and  $g(x)$ is a nonzero polynomial.  Then there exist unique polynomials $q(x), r(x) \\in F[x]$ such that</p><div class=\"displaymath\">\n\\begin{equation*}\nf(x) = g(x) q(x) + r(x),\n\\end{equation*}\n</div><p>where either  $\\deg r(x) \\lt \\deg g(x)$ or $r(x)$ is the zero polynomial.</p></article><article class=\"proof\" id=\"proof-119\"><h6 class=\"heading\"><span class=\"type\">Proof</span></h6><p id=\"p-2579\">We will first consider the existence of $q(x)$ and $r(x)\\text{.}$  If $f(x)$ is the zero polynomial, then</p><div class=\"displaymath\">\n\\begin{equation*}\n0 = 0 \\cdot g(x) + 0;\n\\end{equation*}\n</div><p>hence, both $q$ and $r$ must also be the zero polynomial.  Now suppose that $f(x)$ is not the zero polynomial and that $\\deg f(x) = n$ and $\\deg g(x) = m\\text{.}$   If $m \\gt n\\text{,}$ then we can let $q(x) = 0$ and $r(x) = f(x)\\text{.}$  Hence, we may assume that $m  \\leq n$ and proceed by induction on $n\\text{.}$   If</p><div class=\"displaymath\">\n\\begin{align*}\nf(x) & = a_n x^n + a_{n-1} x^{n - 1} + \\cdots + a_1 x + a_0\\\\\ng(x) & = b_m x^m + b_{m-1} x^{m - 1} + \\cdots + b_1 x + b_0\n\\end{align*}\n</div><p>the polynomial</p><div class=\"displaymath\">\n\\begin{equation*}\nf'(x) = f(x) - \\frac{a_n}{b_m} x^{n - m} g(x)\n\\end{equation*}\n</div><p>has degree less than $n$ or is the zero polynomial.  By induction, there exist polynomials $q'(x)$ and $r(x)$ such that</p><div class=\"displaymath\">\n\\begin{equation*}\nf'(x) = q'(x) g(x) + r(x),\n\\end{equation*}\n</div><p>where $r(x) = 0$ or the degree of $r(x)$ is less than the degree of $g(x)\\text{.}$  Now let</p><div class=\"displaymath\">\n\\begin{equation*}\nq(x) = q'(x) + \\frac{a_n}{b_m} x^{n - m}.\n\\end{equation*}\n</div><p>Then</p><div class=\"displaymath\">\n\\begin{equation*}\nf(x) = g(x) q(x) + r(x),\n\\end{equation*}\n</div><p>with $r(x)$ the zero polynomial or $\\deg r(x) \\lt \\deg g(x)\\text{.}$</p><p id=\"p-2580\">To show that  $q(x)$ and $r(x)$ are unique, suppose that there exist two other polynomials $q_1(x)$ and $r_1(x)$ such that $f(x) = g(x) q_1(x) + r_1(x)$ with $\\deg r_1(x) \\lt \\deg g(x)$ or $r_1(x) = 0\\text{,}$ so that</p><div class=\"displaymath\">\n\\begin{equation*}\nf(x) = g(x) q(x) + r(x) = g(x) q_1(x) + r_1(x),\n\\end{equation*}\n</div><p>and</p><div class=\"displaymath\">\n\\begin{equation*}\ng(x) [q(x) - q_1(x) ] = r_1(x) - r(x).\n\\end{equation*}\n</div><p>If $q(x) - q_1(x)$ is not the zero polynomial, then</p><div class=\"displaymath\">\n\\begin{equation*}\n\\deg( g(x) [q(x) - q_1(x) ] )= \\deg( r_1(x) - r(x) ) \\geq \\deg g(x).\n\\end{equation*}\n</div><p>However, the degrees of both $r(x)$ and $r_1(x)$ are strictly less than the degree of $g(x)\\text{;}$ therefore, $r(x) = r_1(x)$ and $q(x) = q_1(x)\\text{.}$</p></article></div>"]},
{"cell_type":"markdown", "metadata":{}, "source":["<div class=\"mathbook-content\"><article class=\"example-like\" id=\"example-poly-division\"><h6 class=\"heading\"><span class=\"type\">Example</span><span class=\"codenumber\">17.7</span></h6><p id=\"p-2581\">The division algorithm merely formalizes long division of polynomials, a task we have been familiar with since high school. For example, suppose that we divide $x^3 - x^2 + 2 x - 3$ by $x - 2\\text{.}$</p><div class=\"sidebyside\" id=\"sidebyside-10\"><div class=\"sbsrow\" style=\"margin-left:30%;margin-right:30%;\"><div class=\"sbspanel fixed-width\" style=\"width:100%;justify-content:flex-start;\"><table><tr><td class=\"r m b0 r0 l0 t0 lines\" /><td class=\"r m b0 r0 l0 t0 lines\" /><td class=\"r m b0 r0 l0 t0 lines\" /><td class=\"r m b2 r0 l0 t0 lines\">$x^2$</td><td class=\"r m b2 r0 l0 t0 lines\">$+$</td><td class=\"r m b2 r0 l0 t0 lines\">$x$</td><td class=\"r m b2 r0 l0 t0 lines\">$+$</td><td class=\"r m b2 r0 l0 t0 lines\">$4$</td><td class=\"r m b2 r0 l0 t0 lines\" /><td class=\"r m b2 r0 l0 t0 lines\" /></tr><tr><td class=\"r m b0 r0 l0 t0 lines\">$x$</td><td class=\"r m b0 r0 l0 t0 lines\">$-$</td><td class=\"r m b0 r2 l0 t0 lines\">$2$</td><td class=\"r m b0 r0 l0 t0 lines\">$x^3$</td><td class=\"r m b0 r0 l0 t0 lines\">$-$</td><td class=\"r m b0 r0 l0 t0 lines\">$x^2$</td><td class=\"r m b0 r0 l0 t0 lines\">$+$</td><td class=\"r m b0 r0 l0 t0 lines\">$2x$</td><td class=\"r m b0 r0 l0 t0 lines\">$-$</td><td class=\"r m b0 r0 l0 t0 lines\">$3$</td></tr><tr><td class=\"r m b0 r0 l0 t0 lines\" /><td class=\"r m b0 r0 l0 t0 lines\" /><td class=\"r m b0 r0 l0 t0 lines\" /><td class=\"r m b1 r0 l0 t0 lines\">$x^3$</td><td class=\"r m b1 r0 l0 t0 lines\">$-$</td><td class=\"r m b1 r0 l0 t0 lines\">$2x^2$</td><td class=\"r m b1 r0 l0 t0 lines\" /><td class=\"r m b1 r0 l0 t0 lines\" /><td class=\"r m b1 r0 l0 t0 lines\" /><td class=\"r m b1 r0 l0 t0 lines\" /></tr><tr><td class=\"r m b0 r0 l0 t0 lines\" /><td class=\"r m b0 r0 l0 t0 lines\" /><td class=\"r m b0 r0 l0 t0 lines\" /><td class=\"r m b0 r0 l0 t0 lines\" /><td class=\"r m b0 r0 l0 t0 lines\" /><td class=\"r m b0 r0 l0 t0 lines\">$x^2$</td><td class=\"r m b0 r0 l0 t0 lines\">$+$</td><td class=\"r m b0 r0 l0 t0 lines\">$2x$</td><td class=\"r m b0 r0 l0 t0 lines\">$-$</td><td class=\"r m b0 r0 l0 t0 lines\">$3$</td></tr><tr><td class=\"r m b0 r0 l0 t0 lines\" /><td class=\"r m b0 r0 l0 t0 lines\" /><td class=\"r m b0 r0 l0 t0 lines\" /><td class=\"r m b0 r0 l0 t0 lines\" /><td class=\"r m b0 r0 l0 t0 lines\" /><td class=\"r m b1 r0 l0 t0 lines\">$x^2$</td><td class=\"r m b1 r0 l0 t0 lines\">$-$</td><td class=\"r m b1 r0 l0 t0 lines\">$2x$</td><td class=\"r m b1 r0 l0 t0 lines\" /><td class=\"r m b1 r0 l0 t0 lines\" /></tr><tr><td class=\"r m b0 r0 l0 t0 lines\" /><td class=\"r m b0 r0 l0 t0 lines\" /><td class=\"r m b0 r0 l0 t0 lines\" /><td class=\"r m b0 r0 l0 t0 lines\" /><td class=\"r m b0 r0 l0 t0 lines\" /><td class=\"r m b0 r0 l0 t0 lines\" /><td class=\"r m b0 r0 l0 t0 lines\" /><td class=\"r m b0 r0 l0 t0 lines\">$4x$</td><td class=\"r m b0 r0 l0 t0 lines\">$-$</td><td class=\"r m b0 r0 l0 t0 lines\">$3$</td></tr><tr><td class=\"r m b0 r0 l0 t0 lines\" /><td class=\"r m b0 r0 l0 t0 lines\" /><td class=\"r m b0 r0 l0 t0 lines\" /><td class=\"r m b0 r0 l0 t0 lines\" /><td class=\"r m b0 r0 l0 t0 lines\" /><td class=\"r m b0 r0 l0 t0 lines\" /><td class=\"r m b0 r0 l0 t0 lines\" /><td class=\"r m b1 r0 l0 t0 lines\">$4x$</td><td class=\"r m b1 r0 l0 t0 lines\">$-$</td><td class=\"r m b1 r0 l0 t0 lines\">$8$</td></tr><tr><td class=\"r m b0 r0 l0 t0 lines\" /><td class=\"r m b0 r0 l0 t0 lines\" /><td class=\"r m b0 r0 l0 t0 lines\" /><td class=\"r m b0 r0 l0 t0 lines\" /><td class=\"r m b0 r0 l0 t0 lines\" /><td class=\"r m b0 r0 l0 t0 lines\" /><td class=\"r m b0 r0 l0 t0 lines\" /><td class=\"r m b0 r0 l0 t0 lines\" /><td class=\"r m b0 r0 l0 t0 lines\" /><td class=\"r m b0 r0 l0 t0 lines\">$5$</td></tr></table></div></div></div><p id=\"p-2582\">Hence, $x^3 - x^2 + 2 x - 3 = (x - 2) (x^2 + x + 4 ) + 5\\text{.}$</p></article></div>"]},
{"cell_type":"markdown", "metadata":{}, "source":["<div class=\"mathbook-content\"><p id=\"p-2583\">Let $p(x)$ be a polynomial in $F[x]$ and $\\alpha \\in F\\text{.}$  We say that $\\alpha$ is a <dfn class=\"terminology\">zero</dfn> or <dfn class=\"terminology\">root</dfn> of $p(x)$ if $p(x)$ is in the kernel of the evaluation homomorphism $\\phi_{\\alpha}\\text{.}$ All we are really saying here is that $\\alpha$ is a zero of $p(x)$ if $p(\\alpha) = 0\\text{.}$</p></div>"]},
{"cell_type":"markdown", "metadata":{}, "source":["<div class=\"mathbook-content\"><article class=\"theorem-like\" id=\"corollary-poly-factor\"><h6 class=\"heading\"><span class=\"type\">Corollary</span><span class=\"codenumber\">17.8</span></h6><p id=\"p-2584\">Let $F$ be a field. An element $\\alpha \\in F$ is a zero of $p(x) \\in F[x]$ if and only if $x - \\alpha$ is a factor of $p(x)$ in $F[x]\\text{.}$</p></article><article class=\"proof\" id=\"proof-120\"><h6 class=\"heading\"><span class=\"type\">Proof</span></h6><p id=\"p-2585\">Suppose that $\\alpha \\in F$ and $p( \\alpha ) = 0\\text{.}$ By the division algorithm, there exist polynomials $q(x)$ and $r(x)$ such that</p><div class=\"displaymath\">\n\\begin{equation*}\np(x) = (x -\\alpha) q(x) + r(x)\n\\end{equation*}\n</div><p>and the degree of $r(x)$ must be less than the degree of $x -\\alpha\\text{.}$ Since the degree of $r(x)$ is less than 1, $r(x) = a$ for $a \\in F\\text{;}$ therefore,</p><div class=\"displaymath\">\n\\begin{equation*}\np(x) = (x -\\alpha) q(x) + a.\n\\end{equation*}\n</div><p>But</p><div class=\"displaymath\">\n\\begin{equation*}\n0 = p(\\alpha) = 0 \\cdot q(\\alpha) + a = a;\n\\end{equation*}\n</div><p>consequently, $p(x) = (x - \\alpha) q(x)\\text{,}$ and $x - \\alpha$ is a factor  of $p(x)\\text{.}$</p><p id=\"p-2586\">Conversely, suppose that $x - \\alpha$ is a factor of $p(x)\\text{;}$ say $p(x) = (x - \\alpha) q(x)\\text{.}$ Then $p( \\alpha ) = 0 \\cdot q(\\alpha) = 0\\text{.}$</p></article></div>"]},
{"cell_type":"markdown", "metadata":{}, "source":["<div class=\"mathbook-content\"><article class=\"theorem-like\" id=\"corollary-poly-zeros\"><h6 class=\"heading\"><span class=\"type\">Corollary</span><span class=\"codenumber\">17.9</span></h6><p id=\"p-2587\">Let $F$ be a field. A nonzero polynomial $p(x)$ of degree $n$ in $F[x]$ can have at most $n$ distinct zeros in $F\\text{.}$</p></article><article class=\"proof\" id=\"proof-121\"><h6 class=\"heading\"><span class=\"type\">Proof</span></h6><p id=\"p-2588\">We will use induction on the degree of $p(x)\\text{.}$ If $\\deg p(x) = 0\\text{,}$ then $p(x)$ is a constant polynomial and has no zeros.  Let $\\deg p(x) = 1\\text{.}$ Then $p(x) = ax +b$ for some $a$ and $b$ in $F\\text{.}$ If $\\alpha_1$ and $\\alpha_2$ are zeros of $p(x)\\text{,}$ then $a\\alpha_1 + b = a\\alpha_2 +b$ or $\\alpha_1 = \\alpha_2\\text{.}$</p><p id=\"p-2589\">Now assume that $\\deg p(x) \\gt 1\\text{.}$ If $p(x)$ does not have a zero in $F\\text{,}$ then we are done. On the other hand, if $\\alpha$ is a zero of $p(x)\\text{,}$ then $p(x) = (x - \\alpha ) q(x)$ for some $q(x) \\in F[x]$ by Corollary <a href=\"section-poly-division-algorithm.ipynb#corollary-poly-factor\" class=\"xref\" alt=\"Corollary 17.8 \" title=\"Corollary 17.8 \">17.8</a>. The degree of $q(x)$ is $n-1$ by Proposition <a href=\"section-poly-rings.ipynb#proposition-poly-integral-domain\" class=\"xref\" alt=\"Proposition 17.4 \" title=\"Proposition 17.4 \">17.4</a>. Let $\\beta$ be some other zero of $p(x)$ that is distinct from $\\alpha\\text{.}$ Then $p(\\beta) = (\\beta - \\alpha) q(\\beta) = 0\\text{.}$ Since $\\alpha \\neq \\beta$ and $F$ is a field, $q(\\beta ) = 0\\text{.}$ By our induction hypothesis, $q(x)$ can have at most $n - 1$ zeros in $F$ that are distinct from $\\alpha\\text{.}$ Therefore, $p(x)$ has at most $n$ distinct zeros in $F\\text{.}$</p></article></div>"]},
{"cell_type":"markdown", "metadata":{}, "source":["<div class=\"mathbook-content\"><p id=\"p-2590\">Let $F$ be a field.  A monic polynomial $d(x)$ is a <dfn class=\"terminology\">greatest common divisor</dfn> of polynomials $p(x), q(x) \\in F[x]$ if $d(x)$ evenly divides both $p(x)$ and $q(x)\\text{;}$ and, if for any other polynomial $d'(x)$ dividing both $p(x)$ and $q(x)\\text{,}$  $d'(x) \\mid d(x)\\text{.}$  We write $d(x) = \\gcd( p(x), q( x))\\text{.}$ Two polynomials $p(x)$ and $q(x)$ are <dfn class=\"terminology\">relatively prime</dfn> if $\\gcd(p(x), q(x) ) = 1\\text{.}$</p></div>"]},
{"cell_type":"markdown", "metadata":{}, "source":["<div class=\"mathbook-content\"><article class=\"theorem-like\" id=\"proposition-poly-gcd\"><h6 class=\"heading\"><span class=\"type\">Proposition</span><span class=\"codenumber\">17.10</span></h6><p id=\"p-2591\">Let $F$ be a field and suppose that $d(x)$ is a greatest common divisor of two polynomials $p(x)$ and $q(x)$ in $F[x]\\text{.}$ Then there exist polynomials $r(x)$ and $s(x)$ such that</p><div class=\"displaymath\">\n\\begin{equation*}\nd(x) = r(x) p(x) + s(x) q(x).\n\\end{equation*}\n</div><p>Furthermore, the greatest common divisor of two polynomials is unique.</p></article><article class=\"proof\" id=\"proof-122\"><h6 class=\"heading\"><span class=\"type\">Proof</span></h6><p id=\"p-2592\">Let $d(x)$ be the monic polynomial of smallest degree in the set</p><div class=\"displaymath\">\n\\begin{equation*}\nS = \\{ f(x) p(x) + g(x) q(x) : f(x), g(x) \\in F[x]  \\}.\n\\end{equation*}\n</div><p>We can write $d(x) = r(x) p(x) + s(x) q(x)$ for two polynomials  $r(x)$ and $s(x)$ in $F[x]\\text{.}$ We need to show that $d(x)$ divides both $p(x)$ and $q(x)\\text{.}$ We shall first show that $d(x)$ divides $p(x)\\text{.}$ By the division algorithm, there exist polynomials $a(x)$ and $b(x)$ such that $p(x) = a(x) d(x) + b(x)\\text{,}$ where $b(x)$ is either the zero polynomial or $\\deg b(x) \\lt \\deg d(x)\\text{.}$  Therefore,</p><div class=\"displaymath\">\n\\begin{align*}\nb(x) & = p(x) - a(x) d(x)\\\\\n& = p(x) - a(x)( r(x) p(x) + s(x) q(x)) \\\\\n& = p(x) - a(x) r(x) p(x) - a(x)  s(x) q(x)\\\\\n& = p(x)( 1  - a(x) r(x) ) + q(x) ( - a(x)  s(x) )\n\\end{align*}\n</div><p>is a linear combination of $p(x)$ and $q(x)$ and therefore must be in $S\\text{.}$ However, $b(x)$ must be the zero polynomial since $d(x)$ was chosen to be of smallest degree; consequently, $d(x)$ divides $p(x)\\text{.}$  A symmetric argument shows that $d(x)$ must also divide $q(x)\\text{;}$ hence, $d(x)$ is a common divisor of $p(x)$ and $q(x)\\text{.}$</p><p id=\"p-2593\">To show that $d(x)$ is a greatest common divisor of $p(x)$ and $q(x)\\text{,}$ suppose that $d'(x)$ is another common divisor of $p(x)$ and $q(x)\\text{.}$ We will show that $d'(x) \\mid d(x)\\text{.}$  Since $d'(x)$ is a common divisor of $p(x)$ and $q(x)\\text{,}$ there exist polynomials $u(x)$ and $v(x)$ such that $p(x) = u(x) d'(x)$ and $q(x) = v(x) d'(x)\\text{.}$ Therefore,</p><div class=\"displaymath\">\n\\begin{align*}\nd(x) & = r(x) p(x) + s(x) q(x)\\\\\n& =  r(x) u(x) d'(x) + s(x) v(x) d'(x)\\\\\n& = d'(x) [r(x) u(x) + s(x) v(x)].\n\\end{align*}\n</div><p>Since $d'(x) \\mid d(x)\\text{,}$ $d(x)$ is a greatest common divisor of $p(x)$  and $q(x)\\text{.}$</p><p id=\"p-2594\">Finally, we must show that the greatest common divisor of $p(x)$ and $q(x)$ is unique. Suppose that $d'(x)$ is another greatest common divisor of $p(x)$ and $q(x)\\text{.}$ We have just shown that there exist polynomials $u(x)$ and $v(x)$ in $F[x]$ such that $d(x) = d'(x)[r(x) u(x) + s(x) v(x)]\\text{.}$ Since</p><div class=\"displaymath\">\n\\begin{equation*}\n\\deg d(x) =  \\deg d'(x) + \\deg[r(x) u(x) + s(x) v(x)]\n\\end{equation*}\n</div><p>and $d(x)$ and $d'(x)$ are both greatest common divisors, $\\deg d(x) = \\deg d'(x)\\text{.}$ Since $d(x)$ and $d'(x)$ are both monic polynomials of the same degree, it must be the case that $d(x) =~d'(x)\\text{.}$</p></article></div>"]},
{"cell_type":"markdown", "metadata":{}, "source":["<div class=\"mathbook-content\"><p id=\"p-2595\">Notice the similarity between the proof of Proposition <a href=\"section-poly-division-algorithm.ipynb#proposition-poly-gcd\" class=\"xref\" alt=\"Proposition 17.10 \" title=\"Proposition 17.10 \">17.10</a> and the proof of Theorem <a href=\"section-division-algorithm.ipynb#theorem-integers-gcd\" class=\"xref\" alt=\"Theorem 2.10 \" title=\"Theorem 2.10 \">2.10</a>.</p></div>"]}
],
"nbformat": 4, "nbformat_minor": 0, "metadata": {"kernelspec": {"display_name": "", "name": "sagemath"}, "language_info": {"codemirror_mode": {"name": "ipython", "version": 2}, "file_extension": ".py", "mimetype": "text/x-python", "name": "python", "nbconvert_exporter": "python", "pygments_lexer": "ipython2", "version": "2.7.8"}, "name": "section-poly-division-algorithm.ipynb"}
}